Added proofs of correctness for (1) in_re_set_empty, (2) singleton_xform_corr, (3) empty_xform_corr, (4) union_xform_corr, (5) add_xform_corr.
Still need cat_re_xform_erase and cat_re_xform_corr.

x86model/Model/RESet.v
@@ -62,16 +62,45 @@ Module RESet := MSetAVL.Make REOrderedType.
 Module RESETXFORM <: RESetXform.
   Include RESet.  
 
-  Fixpoint tree_type (t:Raw.tree) : type := 
+  Definition re_xf_pair (ty:type) := {r : regexp & regexp_type r ->> List_t ty}.
+
+  Definition in_re_xform ty (rx : re_xf_pair ty) s (v:interp ty) := 
+    let (r,x) := rx in 
+    exists v', in_regexp r s v' /\ List.In v (xinterp x v').
+
+  Fixpoint tree_to_regexp (t : Raw.tree) : regexp := 
     match t with 
-      | Raw.Leaf => Void_t
-      | Raw.Node i lft r rgt => 
-        Sum_t (tree_type lft) (Sum_t (regexp_type r) (tree_type rgt))
+      | Raw.Leaf => Zero
+      | Raw.Node i lft r rgt => Alt (tree_to_regexp lft) (Alt r (tree_to_regexp rgt))
     end.
 
+  Definition tree_type (t : Raw.tree) : type := 
+    regexp_type (tree_to_regexp t).
+
+  Definition in_tree (t: Raw.tree) (str : list char_t) (v: interp (tree_type t)) := 
+    in_regexp (tree_to_regexp t) str v.
+
+  Definition tree_xf_pair (ty:type) := { t : Raw.tree & tree_type t ->> List_t ty }.
+
+  Definition in_tree_xform ty (tx : tree_xf_pair ty) str (v : interp ty) := 
+    let (t,x) := tx in 
+    exists v', in_tree t str v' /\ List.In v (xinterp x v').
+
   Definition re_set_type (rs : t) : type := tree_type (this rs). 
+
+  Definition in_re_set (rs : t) (str : list char_t) (v : interp (re_set_type rs)) := 
+    in_tree (this rs) str v.
   
-  Definition rs_xf_pair (ty:type) := {rs : t & re_set_type rs ->> ty }.
+  Lemma in_re_set_empty : forall s v, not (in_re_set empty s v).
+  Proof.
+    simpl. intros. destruct v.
+  Qed.
+
+  Definition rs_xf_pair (ty:type) := {rs : t & re_set_type rs ->> List_t ty }.
+
+  Definition in_re_set_xform ty (rx : rs_xf_pair ty) s (v:interp ty) := 
+    let (rs, f) := rx in 
+    exists v', in_re_set rs s v' /\ List.In v (xinterp f v').
 
   Definition empty_xform (ty:type) : rs_xf_pair ty := 
     existT _ empty xzero.
@@ -80,27 +109,75 @@ Module RESETXFORM <: RESetXform.
     auto.
   Qed.
 
+  Lemma empty_xform_corr ty (str : list char_t) (v : interp ty) : 
+    ~ in_re_set_xform (empty_xform ty) str v.
+  Proof.
+    unfold in_re_set_xform. unfold not. crush. destruct x.
+  Qed.
+
   Definition singleton_xform (r:regexp) : rs_xf_pair (regexp_type r) := 
-    existT _ (singleton r) (xmatch xzero (xmatch xid xzero)).
+    existT _ (singleton r) (xcons (xmatch xzero (xmatch xid xzero)) xempty).
 
   Lemma singleton_xform_erase : forall r, projT1 (@singleton_xform r) = (singleton r).
     auto.
   Qed.
 
+  Lemma singleton_xform_corr : forall r s v, 
+    in_re_set_xform (singleton_xform r) s v <-> in_regexp r s v.
+  Proof.
+    unfold in_re_set_xform. simpl. crush. destruct x. destruct v.
+    destruct s0. unfold in_re_set, in_tree in H. simpl in H. 
+    repeat in_regexp_inv. destruct v.
+    exists (inr (inl v)). unfold in_re_set, in_tree. simpl.
+    eauto.
+  Qed.
+
   Open Scope Z_scope.
 
   (* These definitions parallel those in the Raw module, but add in an xform. *)
-  Definition create_xform t (l:Raw.tree) (fl : tree_type l ->> t)
-                            (x:regexp) (fx : regexp_type x ->> t)
-                            (r:Raw.tree) (fr : tree_type r ->> t) : 
-    { s : Raw.tree & tree_type s ->> t } := 
+  Definition create_xform ty (l:Raw.tree) (fl : tree_type l ->> List_t ty)
+                             (x:regexp) (fx : regexp_type x ->> List_t ty)
+                             (r:Raw.tree) (fr : tree_type r ->> List_t ty) : 
+    tree_xf_pair ty := 
     existT _ (Raw.Node (Int.Z_as_Int.plus (Int.Z_as_Int.max (Raw.height l) 
                                                             (Raw.height r)) 1)
                        l x r) (xmatch fl (xmatch fx fr)).
 
   Lemma create_xform_erase : 
-    forall t l fl x fx r fr, projT1 (@create_xform t l fl x fx r fr) = Raw.create l x r.
+    forall ty l fl x fx r fr, projT1 (@create_xform ty l fl x fx r fr) = Raw.create l x r.
     auto.
+  Qed.
+
+  Opaque xcross xmap xapp xcomp xmatch xflatten.
+
+  Ltac xmatch_simpl_hyp := 
+    repeat 
+      match goal with
+        | [ H : context[xinterp (xmatch ?f1 ?f2) ?v] |- _ ] => 
+          rewrite (xmatch_corr f1 f2) in H ; simpl in H
+        | [H:context[xcomp ?X1 ?X2] |- _] => 
+          rewrite (xcomp_corr X1 X2) in H ; simpl in H
+      end.
+
+  Ltac xmatch_simpl := 
+    repeat
+      match goal with
+        | [ |- context[xinterp (xmatch ?f1 ?f2) ?v] ] => 
+          rewrite (xmatch_corr f1 f2) ; simpl
+        | [|- context[xcomp ?X1 ?X2]] => rewrite (xcomp_corr X1 X2); simpl
+      end.
+
+  Lemma create_xform_corr ty l fl x fx r fr str v : 
+    in_tree_xform (@create_xform ty l fl x fx r fr) str v <-> 
+    in_tree_xform (existT _ l fl) str v \/
+    in_re_xform (existT _ x fx) str v \/
+    in_tree_xform (existT _ r fr) str v.
+  Proof.
+    simpl. unfold in_tree. crush.
+    repeat in_regexp_inv ; xmatch_simpl_hyp ; crush.
+    econstructor ; crush ; xmatch_simpl ; crush.
+    econstructor ; crush ; xmatch_simpl ; crush.
+    econstructor ; crush ; xmatch_simpl ; crush.
   Qed.
 
   Definition assert_false_xform := create_xform.
@@ -111,10 +188,19 @@ Module RESETXFORM <: RESetXform.
     auto.
   Qed.
 
+  Lemma assert_false_xform_corr ty l fl x fx r fr str v : 
+    in_tree_xform (@create_xform ty l fl x fx r fr) str v <-> 
+    in_tree_xform (existT _ l fl) str v \/
+    in_re_xform (existT _ x fx) str v \/
+    in_tree_xform (existT _ r fr) str v.
+  Proof.
+    apply (create_xform_corr l fl x fx r fr str v).
+  Qed.
+
   Definition bal_xform t (l:Raw.tree) (fl : tree_type l ->> List_t t)
                          (x:regexp) (fx : regexp_type x ->> List_t t)
                          (r:Raw.tree) (fr : tree_type r ->> List_t t) : 
-                         {s : Raw.tree & tree_type s ->> List_t t} := 
+    tree_xf_pair t :=
     let hl := Raw.height l in 
     let hr := Raw.height r in 
     if Int.Z_as_Int.gt_le_dec hl (Int.Z_as_Int.plus hr 2) then
@@ -222,6 +308,80 @@ Module RESETXFORM <: RESetXform.
     apply create_xform_erase.
   Qed.
 
+  Lemma bal_xform_corr1 ty l fl x fx r fr str v : 
+    in_tree_xform (@bal_xform ty l fl x fx r fr) str v -> 
+    in_tree_xform (existT _ l fl) str v \/ 
+    in_re_xform (existT _ x fx) str v \/
+    in_tree_xform (existT _ r fr) str v.
+  Proof.
+    Ltac reduce_if_hyp := 
+    match goal with 
+      | [ H : context[if ?e then _ else _] |- _ ] => destruct e
+    end.
+
+    simpl ; unfold bal_xform ; intros. reduce_if_hyp.
+    destruct l. generalize (proj1 (assert_false_xform_corr _ _ _ _ _ _ _ _) H). crush.
+    reduce_if_hyp. 
+    unfold create_xform in H. simpl in H. unfold in_tree in *. crush.
+    (repeat in_regexp_inv) ; xmatch_simpl_hyp ; crush ; left ; econstructor ; crush.
+    destruct l2. generalize (proj1 (assert_false_xform_corr _ _ _ _ _ _ _ _) H). crush.
+    unfold create_xform in H. simpl in H. unfold in_tree in *. crush.
+    (repeat in_regexp_inv) ; xmatch_simpl_hyp ; crush. left ; crush. 
+    left ; econstructor ; crush. left ; econstructor ; crush. left ; econstructor ; crush.
+    reduce_if_hyp. destruct r.
+    generalize (proj1 (assert_false_xform_corr _ _ _ _ _ _ _ _) H). crush.
+    reduce_if_hyp. unfold create_xform in H. simpl in H.
+    unfold in_tree in *. crush. repeat in_regexp_inv ; xmatch_simpl_hyp ; crush.
+    right ; right ; crush. right ; right ; crush. right ; right ; crush.
+    destruct r1.
+    generalize (proj1 (assert_false_xform_corr _ _ _ _ _ _ _ _) H) ; crush.
+    unfold create_xform in H. unfold in_tree in *. crush. unfold in_tree in *.
+    crush. (repeat in_regexp_inv) ; xmatch_simpl_hyp ; crush. 
+    right ; right ; crush. right ; right ; econstructor ; crush.
+    right ; right ; econstructor ; split ; crush. right ; right ; econstructor ; 
+    split ; crush. right ; right ; econstructor ; split ; crush.
+    generalize (proj1 (create_xform_corr _ _ _ _ _ _ _ _) H) ; crush.
+  Qed.
+
+  Lemma bal_xform_corr2 ty l fl x fx r fr str v : 
+    in_tree_xform (existT _ l fl) str v \/ 
+    in_re_xform (existT _ x fx) str v \/ 
+    in_tree_xform (existT _ r fr) str v -> 
+    in_tree_xform (@bal_xform ty l fl x fx r fr) str v.
+  Proof.
+    unfold bal_xform. intros. 
+    repeat match goal with [ |- in_tree_xform (if ?e then _ else _) _ _] => destruct e end.
+    destruct l. apply assert_false_xform_corr. auto.
+    match goal with [ |- in_tree_xform ((if ?e then _ else _) _) _ _ ] => destruct e end.
+    unfold create_xform ; crush ; unfold in_tree in * ; crush ; repeat in_regexp_inv ; 
+    econstructor ; split ; eauto ; xmatch_simpl ; crush.
+    destruct l2. 
+    unfold assert_false_xform ; crush ; unfold in_tree in * ; crush ; repeat in_regexp_inv ;
+    econstructor ; split ; eauto ; xmatch_simpl ; crush.
+    unfold create_xform ; simpl. unfold in_tree_xform in *. unfold in_tree in *.
+    simpl in *. crush; repeat in_regexp_inv ; econstructor ; split ; eauto ; 
+    xmatch_simpl ; crush.
+    destruct r. apply assert_false_xform_corr ; auto.
+    match goal with [ |- in_tree_xform ((if ?e then _ else _) _) _ _] => destruct e end.
+    unfold create_xform. unfold in_tree_xform in *. unfold in_tree in *. simpl in *.
+    crush ; (repeat in_regexp_inv) ; econstructor ; split ; eauto ; 
+    xmatch_simpl ; crush.
+    destruct r1. apply assert_false_xform_corr ; auto.
+    unfold create_xform. unfold in_tree_xform in *. unfold in_tree in *. simpl in *.
+    crush ; (repeat in_regexp_inv) ; econstructor ; split ; eauto ; 
+    xmatch_simpl ; crush.
+    apply create_xform_corr ; auto.
+  Qed.
+
+  Lemma bal_xform_corr ty l fl x fx r fr str v : 
+    in_tree_xform (existT _ l fl) str v \/ 
+    in_re_xform (existT _ x fx) str v \/ 
+    in_tree_xform (existT _ r fr) str v <-> 
+    in_tree_xform (@bal_xform ty l fl x fx r fr) str v.
+  Proof.
+    intros. split. apply bal_xform_corr2. apply bal_xform_corr1.
+  Qed.    
+
   Lemma cmp_leib : forall r1 r2, REOrderedTypeAlt.compare r1 r2 = Eq -> r1 = r2.
     apply compare_re_eq_leibniz.
   Qed.
@@ -276,13 +436,136 @@ Module RESETXFORM <: RESetXform.
         | [ |- projT1 (match ?e with | existT _ _ => _ end) = _ ] => remember e as e1
     end.
     destruct e1. rewrite bal_xform_erase. 
-    fold tree_type in IHs1. rewrite <- Heqe1 in IHs1. rewrite <- IHs1. auto.
+    fold tree_type in IHs1. 
+    fold regexp_type in IHs1. fold tree_to_regexp in IHs1.
+    unfold tree_type in IHs1, Heqe1. 
+    rewrite <- Heqe1 in IHs1. rewrite <- IHs1. auto.
     specialize (IHs2 x f1 (xcomp (xcomp xinr xinr) f)).
-    fold tree_type in IHs2.
+    fold regexp_type in IHs2. fold tree_to_regexp in IHs2. 
+    unfold tree_type in *.
     match goal with 
       | [ |- projT1 (match ?e with | existT _ _ => _ end) = _ ] => remember e as e1
     end.
     destruct e1. rewrite bal_xform_erase. rewrite <- IHs2. auto.
+  Qed.
+
+  Ltac xinterp_simpl :=
+  repeat match goal with
+    | [|- context[xinterp (xmatch ?X1 ?X2) ?v]] => rewrite (xmatch_corr X1 X2); simpl
+    | [H:context[xinterp (xmatch ?X1 ?X2) ?v] |- _ ] => 
+      rewrite (xmatch_corr X1 X2) in H ; simpl
+    | [|- context[xcomp ?X1 ?X2]] => rewrite (xcomp_corr X1 X2); simpl
+    | [H:context[xcomp ?X1 ?X2] |- _] => 
+      rewrite (xcomp_corr X1 X2) in H; simpl in H
+    | [|- context[xinterp (xpair _ _) _]] => rewrite xpair_corr; simpl
+    | [H:context[xinterp (xpair _ _) _] |- _] => 
+      rewrite xpair_corr in H; simpl in H
+(*
+    | [|- context[xinterp xcross _]] => rewrite xcross_corr; simpl
+    | [H:context[xinterp xcross _] |- _] => 
+      rewrite xcross_corr in H; simpl in H
+*)
+    | [|- context [xinterp xapp (_,_)]] => rewrite xapp_corr; simpl
+    | [H:context [xinterp xapp (_,_)] |- _] => 
+      rewrite xapp_corr in H; simpl in H
+    | [|- context [xinterp (xmap _) ?V]] => 
+      rewrite (@xmap_corr _ _ _ V); simpl
+    | [H:context [xinterp (xmap _) ?V] |- _] => 
+      rewrite (@xmap_corr _ _ _ V) in H; simpl in H
+(*
+    | [|- context[xinterp xflatten _]] => rewrite xflatten_corr2; simpl
+    | [H:context[xinterp xflatten _] |- _] => 
+      rewrite xflatten_corr2 in H; simpl in H
+*)
+  end.
+
+  Lemma add_xform_tree_corr : 
+    forall ty tr ftr x fx str v,
+      in_tree_xform (@add_xform_tree ty x fx tr ftr) str v <-> 
+      in_re_xform (existT _ x fx) str v \/ in_tree_xform (existT _ tr ftr) str v.
+  Proof.
+    induction tr ; intros ; split ; crush.
+    unfold in_tree in H. simpl in H. repeat in_regexp_inv. xmatch_simpl_hyp ; crush.
+    unfold in_tree. simpl. econstructor ; crush. xmatch_simpl ; crush. destruct x0.
+    generalize H ; clear H. generalize (cmp_leib x t1). 
+    generalize (REOrderedTypeAlt.compare x t1). destruct c. intro.
+    generalize (e eq_refl). intro. subst. simpl. crush. unfold in_tree in *.
+    simpl in *. (repeat in_regexp_inv) ; repeat (xinterp_simpl ; crush).
+    generalize (in_app_or _ _ _ H0). crush. right ; econstructor ; crush.
+    right ; econstructor ; crush. intros.
+    specialize (IHtr1 (xcomp xinl ftr) x fx str v) ; clear IHtr2.
+    fold regexp_type in IHtr1. fold tree_to_regexp in IHtr1.
+    unfold tree_type in H.
+    match goal with 
+      | [ H : in_tree_xform (match ?exp with existT _ _ => _ end) _ _ |- _ ] => 
+        remember exp as e1
+    end.
+    destruct e1. generalize (bal_xform_corr1 _ _ _ _ _ _ _ _ H). intros.
+    destruct H0. generalize (proj1 IHtr1 H0). clear IHtr1 H0 H. intro.
+    destruct H. crush. unfold in_tree in *. crush ; xinterp_simpl. crush.
+    crush ; xinterp_simpl ; unfold in_tree in * ; right ; econstructor ; crush.
+    intros. specialize (IHtr2 (xcomp (xcomp xinr xinr) ftr) x fx str v). clear IHtr1.
+    fold regexp_type in IHtr2. fold tree_to_regexp in IHtr2. unfold tree_type in H.
+    match goal with 
+      | [ H : in_tree_xform (match ?exp with existT _ _ => _ end) _ _ |- _ ] => 
+        remember exp as e1
+    end.
+    destruct e1. generalize (bal_xform_corr1 _ _ _ _ _ _ _ _ H) ; intros.
+    destruct H0. crush. xinterp_simpl. unfold in_tree. right ; econstructor ; crush.
+    destruct H0. unfold in_tree. crush. xinterp_simpl. right ; econstructor ; crush.
+    generalize (proj1 IHtr2 H0). clear IHtr2 H0 H. intro. destruct H. crush.
+    unfold in_tree in *. crush. xinterp_simpl. right ; econstructor ; crush.
+    generalize (cmp_leib x t1). generalize (REOrderedTypeAlt.compare x t1).
+    destruct c ; intro. generalize (e eq_refl) ; intro ; subst. simpl. 
+    unfold in_tree. econstructor ; crush. xinterp_simpl. apply in_or_app.
+    right ; auto. specialize (IHtr1 (xcomp xinl ftr) x fx str v). clear IHtr2.
+    fold regexp_type in IHtr1. fold tree_to_regexp in IHtr1. unfold tree_type.
+    match goal with 
+      | [ |- in_tree_xform (match ?exp with existT _ _ => _ end) _ _ ] => 
+        remember exp as e1
+    end.
+    destruct e1. apply bal_xform_corr2. left. apply IHtr1. left. crush.
+    clear IHtr1. specialize (IHtr2 (xcomp (xcomp xinr xinr) ftr) x fx str v).
+    fold regexp_type in IHtr2. fold tree_to_regexp in IHtr2. unfold tree_type.
+    match goal with 
+      | [ |- in_tree_xform (match ?exp with existT _ _ => _ end) _ _ ] => 
+        remember exp as e1
+    end.
+    destruct e1. apply bal_xform_corr2. right. right. apply IHtr2. left ; crush.
+    generalize (cmp_leib x t1). generalize (REOrderedTypeAlt.compare x t1).
+    destruct c ; intros. generalize (e eq_refl) ; intros ; subst. simpl.
+    exists x0. split. auto. xinterp_simpl. destruct x0. xinterp_simpl. auto.
+    xinterp_simpl. destruct s. xinterp_simpl. apply in_or_app. left ; auto.
+    xinterp_simpl ; auto.
+    specialize (IHtr1 (xcomp xinl ftr) x fx str v). clear IHtr2.
+    fold regexp_type in IHtr1. fold tree_to_regexp in IHtr1. unfold tree_type.
+    match goal with 
+      | [ |- in_tree_xform (match ?exp with existT _ _ => _ end) _ _ ] => 
+        remember exp as e1
+    end.
+    destruct e1. apply bal_xform_corr2. unfold in_tree in H. simpl in H.
+    generalize (inv_alt H) ; clear H. intros. destruct H. 
+    destruct H as [v1 [H1 H2]]. subst. left. apply IHtr1. unfold in_tree.
+    right ; econstructor ; split ; eauto. xinterp_simpl. auto.
+    destruct H as [v2 [H1 H2]]. subst. generalize (inv_alt H1). clear H1.
+    intro H1. destruct H1. destruct H as [v1 [H1 H2]]. subst.
+    right ; left. simpl. econstructor ; split ; eauto. xinterp_simpl ; auto.
+    destruct H as [v3 [H1 H2]]. subst. right ; right. simpl. unfold in_tree.
+    econstructor ; split ; eauto ; xinterp_simpl ; auto.
+    clear IHtr1. specialize (IHtr2 (xcomp (xcomp xinr xinr) ftr) x fx str v).
+    fold regexp_type in IHtr2. fold tree_to_regexp in IHtr2. unfold tree_type.
+    match goal with 
+      | [ |- in_tree_xform (match ?exp with existT _ _ => _ end) _ _ ] => 
+        remember exp as e1
+    end.
+    destruct e1. apply bal_xform_corr2. simpl in *. unfold in_tree in *. simpl in *.
+    generalize (inv_alt H) ; clear H ; intro H. destruct H. 
+    destruct H as [v1 [H1 H2]]. subst. left. econstructor ; split ; eauto.
+    xinterp_simpl ; auto. destruct H as [v2 [H1 H2]]. subst.
+    generalize (inv_alt H1) ; clear H1 ; intro H. destruct H.
+    destruct H as [v1 [H1 H2]]. subst. right ; left. econstructor ; split ; eauto.
+    xinterp_simpl ; auto. destruct H as [v3 [H1 H2]]. subst. right ; right.
+    apply IHtr2. right. econstructor. split ; eauto. xinterp_simpl ; auto.
   Qed.
 
   Fixpoint join_xform t (l:Raw.tree) : 
@@ -351,6 +634,77 @@ Module RESETXFORM <: RESetXform.
     rewrite create_xform_erase. auto.
   Qed.
 
+  Lemma join_xform_corr : forall ty l fl x fx r fr str v,
+    in_tree_xform (@join_xform ty l fl x fx r fr) str v <-> 
+      in_tree_xform (existT _ l fl) str v \/ 
+      in_re_xform (existT _ x fx) str v \/ 
+      in_tree_xform (existT _ r fr) str v.
+  Proof.
+    induction l. split. simpl ; intro. 
+    generalize (proj1 (add_xform_tree_corr r fr x fx str v) H). crush.
+    intros. apply add_xform_tree_corr. crush. destruct x0.
+    intros fl x fx. unfold join_xform. fold join_xform.
+    match goal with 
+        [ |- forall _ _ _ _, in_tree_xform (?fexp _ _) _ _ <-> _ ] => 
+        remember fexp as join_aux_xform
+    end.
+    induction r. rewrite Heqjoin_aux_xform. split. intro H.
+    generalize (proj1 (add_xform_tree_corr _ _ _ _ _ _) H). simpl. crush.
+    intros. apply add_xform_tree_corr. crush. destruct x0.
+    rewrite Heqjoin_aux_xform. intros. 
+    split ; intro.
+    destruct (Int.Z_as_Int.gt_le_dec t0 (Int.Z_as_Int.plus t2 Int.Z_as_Int._2)).
+    clear IHl1 IHr1 IHr2. specialize (IHl2 (xcomp (xcomp xinr xinr) fl) x fx
+                                           (Raw.Node t2 r1 t3 r2) fr str v).
+    remember (join_xform l2 (xcomp (xcomp xinr xinr) fl) x fx
+                                   (Raw.Node t2 r1 t3 r2) fr) as e.
+    destruct e. generalize (bal_xform_corr1 _ _ _ _ _ _ _ _ H). clear H.
+    intros. crush ; unfold in_tree ; xinterp_simpl ; crush. left.
+    econstructor ; crush. specialize (H0 (@ex_intro _ _ x2 (conj H H2))).
+    crush. xinterp_simpl. left ; econstructor ; crush.
+    rewrite <- Heqjoin_aux_xform in H.
+    destruct (Int.Z_as_Int.gt_le_dec t2 (Int.Z_as_Int.plus t0 Int.Z_as_Int._2)).
+    specialize (IHr1 (xcomp xinl fr) str v). clear IHl1 IHl2 Heqjoin_aux_xform IHr2.
+    remember (join_aux_xform r1 (xcomp xinl fr)) as e. destruct e.
+    generalize (bal_xform_corr1 _ _ _ _ _ _ _ _ H). clear H. 
+    intros ; crush ; unfold in_tree ; xinterp_simpl ; crush. clear H1.
+    specialize (H0 (ex_intro _ x2 (conj H H2))). crush. xinterp_simpl.
+    right. right. econstructor ; crush. 
+    xinterp_simpl ; right ; right ; econstructor ; crush.
+    xinterp_simpl ; right ; right ; econstructor ; crush.
+    clear Heqjoin_aux_xform IHr1 IHr2 IHl1 IHl2. crush. unfold in_tree in *.
+    crush. repeat in_regexp_inv ; xinterp_simpl ; crush. left ; econstructor ; crush.
+    left ; econstructor ; crush. xinterp_simpl ; right ; left ; econstructor ; crush.
+    xinterp_simpl ; right ; right ; econstructor ; crush.
+    xinterp_simpl ; right ; right ; econstructor ; crush.
+    xinterp_simpl ; right ; right ; econstructor ; crush.
+    rewrite <- Heqjoin_aux_xform.
+    destruct (Int.Z_as_Int.gt_le_dec t0 (Int.Z_as_Int.plus t2 Int.Z_as_Int._2)).
+    specialize (IHl2 (xcomp (xcomp xinr xinr) fl) x fx (Raw.Node t2 r1 t3 r2) fr str v).
+    clear IHl1 Heqjoin_aux_xform IHr1 IHr2.
+    remember (join_xform l2 (xcomp (xcomp xinr xinr) fl) x fx (Raw.Node t2 r1 t3 r2) fr)
+    as e. destruct e. apply bal_xform_corr. crush. unfold in_tree in *. simpl in *.
+    repeat in_regexp_inv ; xinterp_simpl ; crush. left ; econstructor ; split ; eauto.
+    xinterp_simpl ; auto. right ; left ; econstructor ; split ; eauto. 
+    xinterp_simpl ; auto. right. right. apply H1. left ; econstructor ; split ; eauto.
+    xinterp_simpl ; auto. right. right. apply H1. right ; left ; econstructor ; split.
+    eauto. auto. unfold in_tree in *. simpl in *. repeat in_regexp_inv ; xinterp_simpl.
+    right ; right. apply H1. right ; right. econstructor ; crush.
+    right ; right ; apply H1. right ; right ; econstructor ; crush.
+    right ; right ; apply H1. right ; right ; econstructor ; crush.
+    destruct (Int.Z_as_Int.gt_le_dec t2 (Int.Z_as_Int.plus t0 Int.Z_as_Int._2)).
+    clear Heqjoin_aux_xform IHl1 IHl2 IHr2. specialize (IHr1 (xcomp xinl fr) str v).
+    remember (join_aux_xform r1 (xcomp xinl fr)) as e. destruct e.
+    apply bal_xform_corr. crush. unfold in_tree in *. simpl in *.
+    repeat in_regexp_inv ; xinterp_simpl ; crush. left ; apply H1.
+    right ; right ; econstructor ; split ; eauto. xinterp_simpl ; auto.
+    right ; left ; econstructor ; split ; eauto ; xinterp_simpl ; auto.
+    right ; right ; econstructor ; split ; eauto ; xinterp_simpl ; auto.
+    clear Heqjoin_aux_xform IHl1 IHl2 IHr1 IHr2. 
+    crush ; unfold in_tree in * ; simpl in * ; repeat in_regexp_inv ; 
+    xinterp_simpl ; crush ; econstructor ; split ; eauto ; xinterp_simpl ; auto.
+  Qed.
+ 
   Record triple_xform (t:type) (x:regexp) : Type := 
     mkTX { t_left : Raw.tree ; t_left_xform : tree_type t_left ->> List_t t ; 
            t_in : option (regexp_type x ->> List_t t) ; 
@@ -419,7 +773,104 @@ Module RESETXFORM <: RESetXform.
     destruct e1. 
     replace x0 with (projT1 (existT (fun rs => tree_type rs->>List_t t0) x0 x1)) ; auto.
     rewrite Heqe1. rewrite join_xform_erase. destruct t_in0 ; auto.
-  Qed.    
+  Qed.
+
+  Definition in_triple_xform ty x (trip : @triple_xform ty x) str v := 
+    in_tree_xform (existT _ (t_left trip) (t_left_xform trip)) str v \/ 
+    in_tree_xform (existT _ (t_right trip) (t_right_xform trip)) str v \/ 
+    match (t_in trip) with 
+      | Some f => in_re_xform (existT _ x f) str v
+      | None => False
+    end.
+
+  Lemma split_xform_corr : forall ty x s f str v,
+    in_triple_xform (@split_xform ty x s f) str v <-> 
+    in_tree_xform (existT _ s f) str v.
+  Proof.
+    induction s ;  intros. 
+    unfold in_triple_xform ; crush ; unfold tree_type in * ; crush ; 
+    match goal with [ v : void |- _ ] => destruct v end. 
+    simpl. split. generalize (cmp_leib x t1). 
+    generalize (REOrderedTypeAlt.compare x t1). destruct c. intro e.
+    generalize (e eq_refl). intros ; subst. unfold in_tree. 
+    unfold in_triple_xform in H. crush ; xinterp_simpl ; crush. 
+    intros. specialize (IHs1 (xcomp xinl f) str v).
+    remember (split_xform x s1 (xcomp xinl f)) as e1. destruct e1.
+    generalize (join_xform_corr t_right0 t_right_xform0 t1 
+                                (xcomp (xcomp xinl xinr) f) s2 
+                                (xcomp (xcomp xinr xinr) f) str v). intro.
+    remember (join_xform t_right0 t_right_xform0 t1 
+                         (xcomp (xcomp xinl xinr) f) s2 
+                                (xcomp (xcomp xinr xinr) f)) as e1.
+    destruct e1. 
+    unfold in_triple_xform in *.  simpl in *. destruct H.
+    generalize (proj1 IHs1 (@or_introl _ _ H)). crush. xinterp_simpl. simpl.
+    unfold in_tree. econstructor ; split ; eauto. simpl. eauto.
+    destruct H. generalize (proj1 H0 H). clear H0 ; intro H0.
+    destruct H0. generalize (proj1 IHs1 (@or_intror _ _ (@or_introl _ _ H0))).
+    crush. xinterp_simpl. crush. unfold in_tree. simpl. econstructor ; split ; eauto.
+    destruct H0. crush ; xinterp_simpl. unfold in_tree. simpl. econstructor ; split ;
+    crush. crush ; xinterp_simpl ; unfold in_tree ; simpl. econstructor ; crush.
+    destruct t_in0 ; [ idtac | crush]. 
+    specialize (proj1 IHs1 (@or_intror _ _ (@or_intror _ _ H))). crush.
+    unfold in_tree. xinterp_simpl. crush.
+    specialize (IHs2 (xcomp (xcomp xinr xinr) f) str v). clear IHs1. intros.
+    remember (split_xform x s2 (xcomp (xcomp xinr xinr) f)) as e1. destruct e1.
+    generalize (proj1 (join_xform_corr s1 (xcomp xinl f) t1 (xcomp (xcomp xinl xinr) f)
+                                       t_left0 t_left_xform0 str v)). intros.
+    remember (join_xform s1 (xcomp xinl f) t1 (xcomp (xcomp xinl xinr) f)
+                         t_left0 t_left_xform0) as e1 ; destruct e1.
+    unfold in_triple_xform in * ; simpl in *. destruct H.
+    generalize (H0 H). clear H0. intro. destruct H0. 
+    unfold in_tree in * ; xinterp_simpl ; crush. xinterp_simpl ; econstructor ; crush.
+    destruct H0. unfold in_tree. crush ; xinterp_simpl. crush.
+    generalize (proj1 IHs2 (@or_introl _ _ H0)). 
+    unfold in_tree ; crush ; xinterp_simpl ; crush.
+    destruct H. specialize (proj1 IHs2 (@or_intror _ _ (@or_introl _ _ H))).
+    unfold in_tree ; crush ; xinterp_simpl ; crush.
+    destruct t_in0 ; [idtac | crush]. 
+    specialize (proj1 IHs2 (@or_intror _ _ (@or_intror _ _ H))). 
+    unfold in_tree ; crush ; xinterp_simpl ; crush.
+    generalize (cmp_leib x t1). generalize (REOrderedTypeAlt.compare x t1). destruct c. 
+    intros. generalize (e eq_refl). intros ; subst. unfold in_triple_xform. crush.
+    unfold in_tree in H ; simpl in H. repeat in_regexp_inv. left.
+    econstructor ; split ; eauto. xinterp_simpl ; auto.
+    right ; right. econstructor ; split ; eauto. xinterp_simpl ; auto.
+    right ; left ; econstructor ; split ; eauto ; xinterp_simpl ; auto.
+    intros. crush. unfold in_tree in H ; simpl in H.
+    specialize (proj2 (IHs1 (xcomp xinl f) str v)). clear IHs1 IHs2. 
+    intros. remember (split_xform x s1 (xcomp xinl f)) as e1. destruct e1.
+    specialize (proj2 (join_xform_corr t_right0 t_right_xform0 t1 
+                                       (xcomp (xcomp xinl xinr) f)
+                                       s2 (xcomp (xcomp xinr xinr) f) str v)). 
+    intros. remember (join_xform t_right0 t_right_xform0 t1 (xcomp (xcomp xinl xinr) f)
+                                 s2 (xcomp (xcomp xinr xinr) f)) as e2. destruct e2.
+    unfold in_triple_xform. simpl. crush.
+    repeat in_regexp_inv. 
+    assert (exists v', in_tree s1 str v' /\ List.In v (xinterp (xcomp xinl f) v')).
+    econstructor ; split ; eauto. xinterp_simpl. auto. specialize (H1 H3).
+    unfold in_triple_xform in H1. simpl in H1. destruct H1. left ; auto.
+    destruct H1. right ; left. auto. right ; right. auto.
+    right ; left. apply H2. right ; left. econstructor ; split ; eauto.
+    xinterp_simpl. auto. right ; left. apply H2. right ; right. econstructor ; 
+    split ; eauto. xinterp_simpl. auto.
+    intros. specialize (proj2 (IHs2 (xcomp (xcomp xinr xinr) f) str v)).
+    clear IHs1 IHs2. intros. remember (split_xform x s2 (xcomp (xcomp xinr xinr) f)) as e1.
+    destruct e1. specialize (proj2 (join_xform_corr s1 (xcomp xinl f) t1
+                                                    (xcomp (xcomp xinl xinr) f)
+                                                    t_left0 t_left_xform0 str v)). intro.
+    remember (join_xform s1 (xcomp xinl f) t1 (xcomp (xcomp xinl xinr) f) t_left0
+                         t_left_xform0) as e2.
+    destruct e2. unfold in_triple_xform. simpl. unfold in_tree in H. crush.
+    repeat in_regexp_inv. left. apply H1. left ; econstructor ; split ; eauto.
+    xinterp_simpl ; auto. left ; apply H1. right ; left ; econstructor ; split ; eauto ; 
+    xinterp_simpl ; auto. 
+    assert (exists v', in_tree s2 str v' /\ List.In v (xinterp (xcomp (xcomp xinr xinr) f) v')).
+    econstructor ; split ; eauto ; xinterp_simpl ; auto.
+    specialize (H0 H3). unfold in_triple_xform in H0. simpl in H0. 
+    destruct H0. left. apply H1. right ; right. crush.
+    destruct H0 ; auto.
+  Qed.
 
   Fixpoint union_xform_tree t (s1:Raw.tree) : (tree_type s1 ->> List_t t) -> 
                                       forall s2:Raw.tree, tree_type s2 ->> List_t t -> 
@@ -476,9 +927,64 @@ Module RESETXFORM <: RESetXform.
     destruct t_in2 ; injection Heqe2 ; intros ; subst ; auto.
   Qed.
 
+  Lemma union_xform_tree_corr : 
+    forall ty s1 f1 s2 f2 str v, 
+      in_tree_xform (@union_xform_tree ty s1 f1 s2 f2) str v <->
+      in_tree_xform (existT _ s1 f1) str v \/ in_tree_xform (existT _ s2 f2) str v.
+  Proof.
+    induction s1.
+    intros. simpl. crush. destruct x. 
+    intros. destruct s2. simpl. crush. destruct x.
+    unfold union_xform_tree. fold union_xform_tree.
+    generalize (split_xform_corr t1 (Raw.Node t2 s2_1 t3 s2_2) f2 str v).
+    intro. remember (split_xform t1 (Raw.Node t2 s2_1 t3 s2_2) f2) as e.
+    destruct e. unfold in_triple_xform in H. simpl in H.
+    specialize (IHs1_1 (xcomp xinl f1) t_left0 t_left_xform0 str v).
+    remember (union_xform_tree s1_1 (xcomp xinl f1) t_left0 t_left_xform0) as e1.
+    destruct e1.
+    specialize (IHs1_2 (xcomp (xcomp xinr xinr) f1) t_right0 t_right_xform0 str v).
+    remember (union_xform_tree s1_2 (xcomp (xcomp xinr xinr) f1) t_right0 
+                               t_right_xform0) as e2.
+    destruct e2. 
+    match goal with 
+      | [ |- in_tree_xform (join_xform ?x ?x0 ?t1 ?e ?x1 ?x2) ?str ?v <-> _ ] => 
+        generalize (join_xform_corr x x0 t1 e x1 x2 str v) ; intro
+    end.
+    split ; intro.
+    specialize (proj1 H0 H1). clear H0 H1. intro.
+    destruct H0.
+    specialize (proj1 IHs1_1 H0). intro. simpl in *. unfold in_tree in *. simpl in *.
+    crush. xinterp_simpl. left ; econstructor ; crush.
+    destruct H0. destruct t_in0. simpl in *. unfold in_tree. simpl in *.
+    crush. xinterp_simpl. generalize (in_app_or _ _ _ H6).  crush.
+    left ; econstructor ; crush.
+    assert (exists v', in_regexp t1 str v' /\ List.In v (xinterp x3 v')).
+    crush. specialize (H (@or_intror _ _ (@or_intror _ _ H8))). unfold in_tree in H.
+    crush. left. crush. unfold in_tree ; crush. xinterp_simpl. crush.
+    specialize (proj1 IHs1_2 H0). intro. destruct H1. left. 
+    simpl in * ; unfold in_tree in * ; crush. xinterp_simpl ; crush. clear Heqe Heqe2 Heqe1.
+    specialize (proj1 H (@or_intror _ _ (@or_introl _ _ H1))). clear H H1. intro. 
+    right ; auto. clear Heqe Heqe1 Heqe2.
+    apply H0. clear H0. 
+    destruct H1.
+      simpl in *. unfold in_tree in *. crush. repeat in_regexp_inv.
+      assert (exists v', in_tree s1_1 str v' /\ List.In v (xinterp (xcomp xinl f1) v')).
+      econstructor ; split ; eauto. xinterp_simpl. auto.
+      specialize (H5 (@or_introl _ _ H7)). left ; auto. right ; left.
+      econstructor ; split ; eauto. destruct t_in0. xinterp_simpl.
+      apply in_or_app. auto. xinterp_simpl. auto.
+      right ; right ; apply H3. left. econstructor ; split ; eauto ; xinterp_simpl ; auto.
+
+      specialize (proj2 H H0). clear H H0. intros. destruct H.
+      specialize (proj2 IHs1_1 (@or_intror _ _ H)). clear IHs1_1 H. intro. auto.
+      destruct H. specialize (proj2 IHs1_2 (@or_intror _ _ H)). clear IHs1_2 H. auto.
+      destruct t_in0 ; [idtac | crush]. right ; left. crush.
+      econstructor ; split ; eauto. xinterp_simpl. apply in_or_app. auto.
+  Qed.
+
   (* should rewrite using explicit code -- hard to work with it this way... *)
   Definition add_xform (ty:type)(x:regexp)(fx:regexp_type x->>List_t ty)
-             (rs:rs_xf_pair (List_t ty)) : rs_xf_pair (List_t ty).
+             (rs:rs_xf_pair ty) : rs_xf_pair ty.
     destruct rs as [s fs].
     destruct s as [t ok].
     remember (add_xform_tree x fx t fs) as p.
@@ -514,8 +1020,22 @@ Module RESETXFORM <: RESetXform.
     rewrite (proof_irrelevance _ o0 (Raw.add_ok x ok)). auto.
   Qed.
 
-  Definition union_xform (ty:type) (rs1 rs2 : rs_xf_pair (List_t ty)) : 
-    rs_xf_pair (List_t ty).
+  Lemma add_xform_corr ty x fx rs str v : 
+    in_re_set_xform (@add_xform ty x fx rs) str v <-> 
+    in_re_xform (existT _ x fx) str v \/ in_re_set_xform rs str v.
+  Proof.
+    destruct rs as [s fs]. destruct s as [t ok]. unfold in_re_set_xform.
+    unfold add_xform. simpl. unfold eq_rec_r, eq_rec, eq_rect. simpl.
+    generalize (eq_ind_r (fun s => Raw.Ok (projT1 s)) 
+                         (eq_ind_r (fun t0 => Raw.Ok t0) (Raw.add_ok x ok)
+                                   (add_xform_tree_erase t x fx fs))).
+    generalize (add_xform_tree_corr t fs x fx str v).
+    remember (add_xform_tree x fx t fs) as p. intros.
+    destruct p. unfold re_set_type. simpl. unfold in_re_set. simpl.
+    apply H.
+  Qed.
+
+  Definition union_xform (ty:type) (rs1 rs2 : rs_xf_pair ty) : rs_xf_pair ty.
     destruct rs1 as [s1 f1].
     destruct rs2 as [s2 f2].
     destruct s1 as [t1 okt1].
@@ -555,26 +1075,82 @@ Module RESETXFORM <: RESetXform.
     rewrite (proof_irrelevance _ o (Raw.union_ok okt1 okt2)). auto.
   Qed.
 
-  (* An iterator for the trees -- extracts the elements and the appropriate
-     transform.  Don't need this now, but I've left it in. *)
-  Section ITER_TREE.
-    Parameter T : type.
-    Parameter A : Type.
-    Parameter comb : forall r, regexp_type r ->> T -> A -> A.
-    Fixpoint iter_tree_xform (s:Raw.tree) : (tree_type s ->> T) -> A -> A := 
-      match s return tree_type s ->> T -> A -> A with
+  Lemma union_xform_corr ty rs1 rs2 str v : 
+    in_re_set_xform (@union_xform ty rs1 rs2) str v <-> 
+    in_re_set_xform rs1 str v \/ in_re_set_xform rs2 str v.
+  Proof.
+    destruct rs1 as [s1 f1].
+    destruct rs2 as [s2 f2].
+    destruct s1 as [t1 okt1].
+    destruct s2 as [t2 okt2]. simpl. 
+    generalize (eq_ind_r
+                    (fun s : {rs : Raw.tree & tree_type rs ->> List_t ty} =>
+                     Raw.Ok (projT1 s))
+                    (eq_ind_r (fun t3 : Raw.tree => Raw.Ok t3)
+                       (Raw.union_ok (s1:=t1) (s2:=t2) okt1 okt2)
+                       (union_xform_tree_erase t1 f1 t2 f2))).
+    generalize (union_xform_tree_corr t1 f1 t2 f2 str v).
+    remember (union_xform_tree t1 f1 t2 f2) as p. intros. 
+    destruct p. simpl. unfold re_set_type, in_re_set. simpl.
+    unfold eq_rec_r, eq_rec, eq_rect. simpl. apply H.
+  Qed.
+
+  Section FOLD_TREE_XFORM.
+    Variable ty : type.
+    Variable A : Type.
+    Variable f : forall r, regexp_type r ->> ty -> A -> A.
+    Fixpoint fold_tree_xform (s:Raw.tree) : (tree_type s ->> ty) -> A -> A := 
+      match s return tree_type s ->> ty -> A -> A with
         | Raw.Leaf => fun _ v => v
         | Raw.Node _ l x r => 
-          fun f v => iter_tree_xform r (xcomp (xcomp xinr xinr) f) 
-                                     (comb x (xcomp (xcomp xinl xinr) f) 
-                                           (iter_tree_xform l (xcomp xinl f) v))
+          fun fs v => fold_tree_xform r (xcomp (xcomp xinr xinr) fs) 
+                                     (f x (xcomp (xcomp xinl xinr) fs) 
+                                           (fold_tree_xform l (xcomp xinl fs) v))
       end.
-  End ITER_TREE.
+  End FOLD_TREE_XFORM.
 
-Print Raw.union.
-Print Raw.split.
-Print Raw.triple.
-Print Raw.join.
+  Definition map_tree_xform ty 
+             (s:Raw.tree) 
+             (fs:tree_type s ->> List_t ty) 
+             (g:forall r:regexp, regexp_type r ->> List_t ty -> 
+                                 {r' : regexp & regexp_type r' ->> List_t ty}) :
+             { s' : Raw.tree & tree_type s' ->> List_t ty } := 
+    fold_tree_xform (fun r fr (sx : {s':Raw.tree & tree_type s' ->> List_t ty}) => 
+                       let (r',fr') := g r fr in
+                       let (s',fs') := sx in 
+                       add_xform_tree r' fr' s fs) s fs 
+                    (existT _ Raw.Leaf xzero).
+
+(* Raw.fold = 
+fix fold (A : Type) (f : Raw.elt -> A -> A) (t : Raw.tree) 
+         (base : A) {struct t} : A :=
+  match t with
+  | Raw.Leaf => base
+  | Raw.Node _ l x r => fold A f r (f x (fold A f l base))
+  end
+     : forall A : Type, (Raw.elt -> A -> A) -> Raw.tree -> A -> A
+*)
+  Lemma map_tree_xform_unfold ty g i l v r fs : 
+    (@map_tree_xform ty (Raw.Node i l v r) fs g) = 
+    let (s1,f1) := @map_tree_xform ty l (xcomp xinl fs) g in 
+    let (v',fv') := g v (xcomp (xcomp xinl xinr) fs) in
+    let (s2,f2) := add_xform_tree v' fv' s1 f1 in 
+    
+
+  Lemma map_tree_xform_erase ty g1 g2 : 
+    (forall r (f:regexp_type r ->> List_t ty), projT1 (g1 r f) = g2 r) -> 
+    forall s fs, 
+    projT1 (@map_tree_xform ty s fs g1) = 
+    Raw.fold (fun r s' => Raw.add (g2 r) s') s Raw.Leaf.
+  Proof.
+    intro H. induction s ; intro. auto. simpl.
+    unfold map_tree_xform. 
+  
+  Definition cat_re_xform : 
+    forall ty, rs_xf_pair (List_t ty) -> 
+               forall r:regexp, rs_xf_pair (Pair_t ty (regexp_type r)).
+
+
 End RESETXFORM.
 
 (* Module RR : WSets := RESet. *)
